Common.v
@@ -8,6 +8,13 @@ Module PS := Coq.MSets.MSetPositive.PositiveSet.
 Module PM := Coq.FSets.FMapPositive.PositiveMap.
 
 Definition ident := positive.
+Definition ident_eq_dec := Pos.eq_dec.
+
+Lemma In_dec:
+  forall x S, {PS.In x S}+{~PS.In x S}.
+Proof.
+  intros i m; unfold PS.In; case (PS.mem i m); auto.
+Qed.
 
 Inductive const : Set :=
 | Cint : BinInt.Z -> const
